backend/Stackingproof.v
@@ -2467,7 +2467,8 @@ Proof.
         rewrite sep_comm, sep_assoc in SEP |- *.
         eapply globalenv_inject_incr; eauto. destruct H12.
         eapply Mem.unchanged_on_support; eauto.
-Qed.
+        admit. admit.
+Admitted.
 
 Lemma wt_prog:
   forall i fd, In (i, Gfun fd) prog.(prog_defs) -> wt_fundef fd.
